\documentclass[a4paper,12pt]{article} % This defines the style of your paper

\usepackage[top = 2.5cm, bottom = 2.5cm, left = 2.5cm, right = 2.5cm]{geometry} 

\usepackage[T1]{fontenc}
\usepackage[utf8]{inputenc}
\usepackage[english]{babel}

\usepackage{multirow} % Multirow is for tables with multiple rows within one cell.
\usepackage{booktabs} % For even nicer tables.

\usepackage{amsmath} 
\usepackage{graphicx}

\newtheorem{definition}{Definition}
\newtheorem{observation}{Observation}[definition]

\usepackage{setspace}
\setlength{\parindent}{0in}
\setlength{\parskip}{.5em}

\begin{document}

\begin{center}
    {\Large \bf Homework 2}
    \vspace{2mm}

    {\bf Jiří Klepl}

\end{center}

\vspace{0.4cm}

\begin{quote}
    (10 points) Let $\varphi$ be a CNF and $C \in \varphi$ a clause in $\varphi$ and $l \in C$ a literal in $C$. We say that $C$ is
blocked by literal $l$ if for every other clause $D \in \varphi$ which contains $\neg l$ we have that $Res_l(C, D)$ is a
tautology (i.e. there is another literal $l_D \in D$ such that $\neg l_D \in C$). Show that $\varphi$ is equisatisfiable with
$\varphi \setminus \{C\}$, i.e. $\varphi$ is satisfiable if and only if $\varphi \setminus \{C\}$ is satisfiable.
\end{quote}

We can rewrite $\varphi$ into $C \wedge \varphi_l \wedge \varphi_{\neg l} \wedge \varphi_r$ where $\varphi_{l}$ contains the clauses other than $C$ that contain $l$; $\varphi_{\neg l}$ contains the clauses that contain $\neg l$; and $\varphi_r$ contains the clauses of $\varphi$ that don't contain neither $l$ nor $\neg l$.


It holds that: $C \wedge \varphi_l \wedge \varphi_{\neg l} \wedge \varphi_r \equiv (\neg l \to (C' \wedge \varphi_l')) \wedge (l \to \varphi_{\neg l}') \wedge \varphi_r$ where $C'$ is the clause $C$ after removing the literal $l$; and $\varphi_l'$ consist of the clauses in $\varphi_l$ after removing the literal $l$; and, similarly, $\varphi_{\neg l}'$ contains the clauses from $\varphi_{\neg l}$ after removing $\neg l$ from each.

And then, since neither of $C'$, $\varphi_l'$, $\varphi_{\neg l}'$, nor $\varphi_r$ contain either of the literals $l$ and $\neg l$, it holds that: $(\neg l \to (C' \wedge \varphi_l')) \wedge (l \to \varphi_{\neg l}') \wedge \varphi_r \equiv_{SAT} ((C' \wedge \varphi_l') \vee \varphi_{\neg l}') \wedge \varphi_r$.

Then, from distributivity of $\vee$ and $\wedge$, we get: $((C' \wedge \varphi_l') \vee \varphi_{\neg l}') \wedge \varphi_r \equiv \bigwedge_{D' \in \varphi_{\neg l}} (C' \vee D') \wedge \bigwedge_{D' \in \varphi_{\neg l}'}(\varphi_l' \vee D') \wedge \varphi_r = \bigwedge_{D \in \varphi_{\neg l}} Res_l(C, D) \wedge \bigwedge_{D' \in \varphi_{\neg l}'}(\varphi_l' \vee D') \wedge \varphi_r \equiv \bigwedge_{D \in \varphi_{\neg l}} Res_l(C, D) \wedge (\varphi_l' \vee \varphi_{\neg l}') \wedge \varphi_r$; the equality follows the definition of $C'$ and $\varphi_{\neg l}'$ from $C$ and $\varphi_{\neg l}$; and the second  equivalence, again, from distributivity of $\vee$ and $\wedge$.

The assignment states that $Res_l(C, D)$ is a tautology for every $D \in \varphi_{\neg l}$, and thus: $\bigwedge_{D \in \varphi_{\neg l}} Res_l(C, D) \wedge (\varphi_l' \vee \varphi_{\neg l}') \wedge \varphi_r \equiv_{SAT} (\varphi_l' \vee \varphi_{\neg l}') \wedge \varphi_r \equiv_{SAT} (\neg l \to \varphi_l') \wedge (l \to \varphi_{\neg l}') \wedge \varphi_r \equiv \varphi_l \wedge \varphi_{\neg l} \wedge \varphi_r = \varphi \setminus \{C\}$.

And thus: $$\varphi \equiv_{SAT} \varphi \setminus \{C\}$$

\end{document}